Make concrete linking much more sensible

doc/coq/simple/LinkSound.v
@@ -6,149 +6,57 @@ Module CL := Linking.
 
 Generalizable Variables BCT BAT ACT AAT.
 
-Definition In_linked_t `{Conc.time BCT} `{Conc.time ACT}
-  (final : BCT) (init : ACT) (t : @link BCT _ ACT _) :=
-  match t with
-  | L bf af =>
-    if leb final bf then
-      eqb final bf = true
-    else
-      eqb init af = true
-  end.
-
-Fixpoint In_linked_ctx `{Conc.time BCT} `{Conc.time ACT}
-  (final : BCT) (init : ACT) (C : @dy_ctx (@link BCT _ ACT _)) :=
-  match C with
-  | [||] => True
-  | dy_binde _ t C' => In_linked_t final init t /\ In_linked_ctx final init C'
-  | dy_bindm _ C' C'' => In_linked_ctx final init C' /\ In_linked_ctx final init C''
-  end.
-
-Definition In_linked_v `{Conc.time BCT} `{Conc.time ACT}
-  (final : BCT) (init : ACT) (v : @expr_value (@link BCT _ ACT _)) :=
-  match v with
-  | Closure _ _ C => In_linked_ctx final init C
-  end.
-
-Definition In_linked_mem `{Conc.time BCT} `{Conc.time ACT}
-  (final : BCT) (init : ACT) (mem : (@link BCT _ ACT _) -> option (@expr_value (@link BCT _ ACT _))) :=
-  forall t,
-    match mem t with
-    | Some v => In_linked_t final init t /\ In_linked_v final init v
-    | None => True
-    end.
-
-Lemma bound_then_lift_in `{Conc.time BCT} `{Conc.time ACT}
-  (final : BCT) (init : ACT) (C : @dy_ctx BCT) (BOUND : dy_ctx_bound C final) :
-  In_linked_ctx final init (lift_ctx_bf init C).
-Proof.
-  induction C; eauto; destruct BOUND as [BOUND1 BOUND2].
-  - simpl. replace (leb final tx) with false.
-    split; try rewrite eqb_eq; eauto.
-    symmetry. refl_bool. intros contra.
-    assert (final = tx) as RR.
-    apply leb_sym. assumption. apply BOUND1. subst.
-    destruct BOUND1 as [? absurd]. rewrite t_refl in *. inversion absurd.
-  - simpl. split; eauto.
-Qed.
-
 Definition link_abs `{Conc.time BCT} `{Abs.time BAT} `{Conc.time ACT} `{Abs.time AAT}
-  (final : BCT) (αbf : BCT -> BAT) (αaf : ACT -> AAT) :=
-  fun t =>
+  (final : BCT) (init : ACT) (αbf : BCT -> BAT) (αaf : ACT -> AAT) :=
+  fun t : link final init =>
   match t with
-  | L bf af =>
-    if leb final bf then AF (αaf af) else BF (αbf bf)
+  | L _ _ bf af _ =>
+    if eqb final bf then AF (αaf af) else BF (αbf bf)
   end.
 
 Lemma trans_ctx_lift `{Conc.time BCT} `{Abs.time BAT} `{Conc.time ACT} `{Abs.time AAT}
   (final : BCT) (init : ACT) (αbf : BCT -> BAT) (αaf : ACT -> AAT) :
-  let αlink := (link_abs final αbf αaf) in
+  let αlink := (link_abs final init αbf αaf) in
   forall C (BOUND : dy_ctx_bound C final),
-    trans_ctx αlink (lift_ctx_bf init C) =
+    trans_ctx αlink (lift_ctx_bf final init C) =
     AL.lift_ctx_bf (trans_ctx αbf C).
 Proof.
   induction C; simpl; eauto; intros [BOUND1 BOUND2].
-  - replace (leb final tx) with false. rewrite IHC; eauto.
+  - replace (eqb final tx) with false. rewrite IHC; eauto.
     symmetry. destruct BOUND1 as [LE NEQ].
-    refl_bool. intros contra. assert (tx = final). apply leb_sym; eauto. subst.
+    refl_bool. intros contra. rewrite eqb_eq in contra. subst.
     rewrite t_refl in NEQ. inversion NEQ.
   - rewrite IHC1; eauto. rewrite IHC2; eauto.
 Qed.
 
 Lemma trans_ctx_filter `{Conc.time BCT} `{Abs.time BAT} `{Conc.time ACT} `{Abs.time AAT}
   (final : BCT) (init : ACT) (αbf : BCT -> BAT) (αaf : ACT -> AAT) :
-  forall C (INC : In_linked_ctx final init C),
-  let αlink := (link_abs final αbf αaf) in
+  forall C,
+  let αlink := (link_abs final init αbf αaf) in
   let eqb' t t' := eqb (αlink t) (αlink t') in
-  trans_ctx αaf (CL.filter_ctx_af final C) = AL.filter_ctx_af (trans_ctx αlink C).
+  trans_ctx αaf (CL.filter_ctx_af final init C) = AL.filter_ctx_af (trans_ctx αlink C).
 Proof.
-  induction C; simpl; eauto; intros [IN1 IN2].
+  induction C; simpl; eauto.
   - destruct tx. simpl in *.
-    destruct (leb final bf); simpl; eauto.
+    destruct (eqb final bf); simpl; eauto.
     rewrite IHC; eauto.
   - rewrite IHC1; eauto. rewrite IHC2; eauto.
-Qed.
-
-Lemma In_linked_ctx_prefix `{Conc.time BCT} `{Conc.time ACT} eqb
-  (final : BCT) (init : ACT) :
-  forall (Cout C : @dy_ctx (@link BCT _ ACT _))
-         (INC : In_linked_ctx final init C),
-  In_linked_ctx final init (delete_prefix eqb Cout C).
-Proof.
-  induction Cout; intros; eauto.
-  - destruct C; eauto. simpl.
-    destruct (eq_eid x x0) eqn:EQid;
-    destruct (eqb tx tx0) eqn:EQt; eauto.
-    simpl in *. apply IHCout; apply INC.
-  - destruct C; eauto. simpl.
-    destruct (eq_mid M M0) eqn:EQid;
-    destruct (eq_ctx eqb Cout1 C1) eqn:EQC; eauto.
-    simpl in *. apply IHCout2; apply INC.
-Qed.
-
-Lemma In_linked_ctx_map_aux `{Conc.time BCT} `{Conc.time ACT} eqb
-  (final : BCT) (init : ACT) :
-  forall n (C Cout : @dy_ctx (@link BCT _ ACT _)) (LE : dy_level C <= n)
-         (INC : In_linked_ctx final init C),
-  In_linked_ctx final init (delete_map eqb Cout C).
-Proof.
-  induction n; intros; induction C; try reflexivity; try (inversion LE; fail).
-  - rewrite delete_map_red_binde. simpl. simpl in INC.
-    split; try apply INC. apply IHC; try apply INC.
-    simpl in LE. nia.
-  - rewrite delete_map_red_bindm. simpl. simpl in INC.
-    split. apply IHn. simpl in *.
-    etransitivity. apply delete_prefix_dec. nia.
-    apply In_linked_ctx_prefix. apply INC.
-    apply IHC2. simpl in LE. nia. apply INC.
-Qed.
-
-Lemma In_linked_ctx_delete `{Conc.time BCT} `{Conc.time ACT} eqb
-  (final : BCT) (init : ACT) :
-  forall (Cout C : @dy_ctx (@link BCT _ ACT _))
-         (INC : In_linked_ctx final init C),
-  In_linked_ctx final init (delete_ctx eqb Cout C).
-Proof.
-  intros. unfold delete_ctx.
-  apply In_linked_ctx_map_aux with (n := dy_level C).
-  apply delete_prefix_dec. apply In_linked_ctx_prefix. eauto.
 Qed.
 
 Lemma trans_ctx_link `{Conc.time BCT} `{Abs.time BAT} `{Conc.time ACT} `{Abs.time AAT}
   (final : BCT) (init : ACT) (Cout : @dy_ctx BCT) (BOUND : dy_ctx_bound Cout final)
   (αbf : BCT -> BAT) (αaf : ACT -> AAT) :
-  forall C (INC : In_linked_ctx final init C),
-  let αlink := (link_abs final αbf αaf) in
+  forall C,
+  let αlink := (link_abs final init αbf αaf) in
   let eqb' t t' := eqb (αlink t) (αlink t') in
   trans_ctx αaf
-    (CL.filter_ctx_af final (delete_ctx eqb' (CL.lift_ctx_bf init Cout) C)) =
+    (CL.filter_ctx_af final init (delete_ctx eqb' (CL.lift_ctx_bf final init Cout) C)) =
   AL.filter_ctx_af
     (delete_ctx eqb (AL.lift_ctx_bf (trans_ctx αbf Cout)) (trans_ctx αlink C)).
 Proof.
   intros.
   rewrite <- trans_ctx_lift with (final := final) (init := init) (αaf := αaf); eauto.
   rewrite <- trans_ctx_delete. rewrite trans_ctx_filter with (init := init) (αbf := αbf). eauto.
-  apply In_linked_ctx_delete. eauto.
 Qed.
 
 Lemma In_map_l {T T'} :
@@ -173,12 +81,11 @@ Lemma trans_mem_link `{Conc.time BCT} `{Abs.time BAT} `{Conc.time ACT} `{Abs.tim
   (final : BCT) (init : ACT) (Cout : @dy_ctx BCT) (BOUND : dy_ctx_bound Cout final)
   (αbf : BCT -> BAT) (αaf : ACT -> AAT) (PRES : preserve_tick αaf) :
   forall mem abs_mem
-    (EQ : trans_mem (link_abs final αbf αaf) mem abs_mem)
-    (INm : In_linked_mem final init mem),
-  let αlink := (link_abs final αbf αaf) in
+    (EQ : trans_mem (link_abs final init αbf αaf) mem abs_mem),
+  let αlink := (link_abs final init αbf αaf) in
   trans_mem αaf
-  (CL.filter_mem_af final
-     (CL.delete_ctx_mem αlink (CL.lift_ctx_bf init Cout) mem))
+  (CL.filter_mem_af final init
+     (CL.delete_ctx_mem αlink (CL.lift_ctx_bf final init Cout) mem))
   (AL.filter_mem_af
      (AL.delete_ctx_mem (AL.lift_ctx_bf (trans_ctx αbf Cout))
         abs_mem)).
@@ -195,85 +102,79 @@ Proof.
     red in EQ. specialize (EQ (AL.AF abs_t) v').
     rewrite EQ in IN.
     destruct IN as [t [v'' [TRANSv [TRANSt ACCESS]]]].
-    specialize (INm t). rewrite ACCESS in INm.
-    destruct INm as [INt INv].
-    destruct t. simpl in INt. simpl in TRANSt.
-    destruct (leb final bf); try (inversion TRANSt; fail).
-    rewrite eqb_eq in INt. subst.
-    exists af. rewrite ACCESS.
-    exists (CL.filter_v_af bf
+    destruct t. simpl in TRANSt.
+    destruct (eqb final bf) eqn:EQt; try (inversion TRANSt; fail).
+    rewrite eqb_eq in EQt. subst.
+    exists af. replace (CL.LINK_pf_af bf init af) with LINK; try apply proof_irrelevance.
+    rewrite ACCESS.
+    exists (CL.filter_v_af bf init
        (delete_ctx_v
-          (fun t t' : link =>
-           eqb (link_abs bf αbf αaf t)
-             (link_abs bf αbf αaf t'))
-          (CL.lift_ctx_bf init Cout) v'')).
+          (fun t t' : link bf init =>
+           eqb (link_abs bf init αbf αaf t)
+             (link_abs bf init αbf αaf t'))
+          (CL.lift_ctx_bf bf init Cout) v'')).
     repeat split; try (inversion TRANSt; eauto; fail).
     destruct v''. simpl.
     rewrite <- trans_ctx_lift with (final := bf) (init := init) (αaf := αaf); eauto.
     assert (delete_ctx AL.link_eqb
-        (trans_ctx (link_abs bf αbf αaf) (lift_ctx_bf init Cout))
-        (trans_ctx (link_abs bf αbf αaf) C) =
-        trans_ctx (link_abs bf αbf αaf) 
-          (delete_ctx (fun t t' => AL.link_eqb ((link_abs bf αbf αaf) t) ((link_abs bf αbf αaf) t'))
-            (lift_ctx_bf init Cout) C)) as RR.
+        (trans_ctx (link_abs bf _ αbf αaf) (lift_ctx_bf _ init Cout))
+        (trans_ctx (link_abs bf _ αbf αaf) C) =
+        trans_ctx (link_abs bf _ αbf αaf) 
+          (delete_ctx (fun t t' => AL.link_eqb ((link_abs bf _ αbf αaf) t) ((link_abs bf _ αbf αaf) t'))
+            (lift_ctx_bf _ init Cout) C)) as RR.
     { symmetry. apply (@trans_ctx_delete _ (@AL.link BAT AAT) _ AL.link_eq). }
     rewrite RR. rewrite trans_ctx_filter with (init := init) (αbf := αbf). eauto.
-    apply In_linked_ctx_delete. eauto.
   - destruct IN as [af [v [TRANSv [TRANSt SOME]]]].
-    destruct (mem (CL.L final af)) eqn:ACCESS; try (inversion SOME; fail).
+    destruct (mem (CL.L _ _ _ af _)) eqn:ACCESS; try (inversion SOME; fail).
     subst. red in EQ.
     destruct e. simpl in *.
     inversion SOME. subst.
     exists (Closure x e
       (delete_ctx ALinking.link_eqb
         (AL.lift_ctx_bf (trans_ctx αbf Cout))
-        (trans_ctx (link_abs final αbf αaf) C))).
+        (trans_ctx (link_abs final init αbf αaf) C))).
     split. simpl.
     rewrite <- trans_ctx_lift with (final := final) (init := init) (αaf := αaf); eauto.
     assert (delete_ctx AL.link_eqb
-        (trans_ctx (link_abs final αbf αaf) (lift_ctx_bf init Cout))
-        (trans_ctx (link_abs final αbf αaf) C) =
-        trans_ctx (link_abs final αbf αaf) 
-          (delete_ctx (fun t t' => AL.link_eqb ((link_abs final αbf αaf) t) ((link_abs final αbf αaf) t'))
-            (lift_ctx_bf init Cout) C)) as RR.
+        (trans_ctx (link_abs final _ αbf αaf) (lift_ctx_bf _ init Cout))
+        (trans_ctx (link_abs final _ αbf αaf) C) =
+        trans_ctx (link_abs final _ αbf αaf) 
+          (delete_ctx (fun t t' => AL.link_eqb ((link_abs final _ αbf αaf) t) ((link_abs final _ αbf αaf) t'))
+            (lift_ctx_bf _ init Cout) C)) as RR.
     { symmetry. apply (@trans_ctx_delete _ (@AL.link BAT AAT) _ AL.link_eq). }
     rewrite RR. rewrite trans_ctx_filter with (init := init) (αbf := αbf). eauto.
-    apply In_linked_ctx_delete. specialize (INm (CL.L final af)). rewrite ACCESS in INm. apply INm.
     rewrite In_map_l.
-    exists (Closure x e (trans_ctx (link_abs final αbf αaf) C)).
+    exists (Closure x e (trans_ctx (link_abs final _ αbf αaf) C)).
     split. eauto.
     rewrite EQ.
-    exists (CL.L final af).
+    exists (CL.L _ _ final af (CL.LINK_pf_af final init af)).
     exists (Closure x e C).
-    split; eauto. split; eauto. simpl. rewrite leb_refl. eauto.
+    split; eauto. split; eauto. simpl. rewrite t_refl. eauto.
 Qed.
 
 Theorem link_abs_pres `{Conc.time BCT} `{Abs.time BAT} `{Conc.time ACT} `{Abs.time AAT}
   (final : BCT) (init : ACT) (Cout : @dy_ctx BCT) (BOUND : dy_ctx_bound Cout final)
   (αbf : BCT -> BAT) (αaf : ACT -> AAT) (PRES : preserve_tick αaf) :
   forall (af : ACT) C mem x v abs_mem
-    (EQ : trans_mem (link_abs final αbf αaf) mem abs_mem)
-    (INm : In_linked_mem final init mem)
-    (INC : In_linked_ctx final init C)
-    (INv : In_linked_v final init v),
-  let αlink := (link_abs final αbf αaf) in
-  αlink (CL.link_tick αlink final init Cout C (ST mem (L final af)) x v) =
+    (EQ : trans_mem (link_abs final init αbf αaf) mem abs_mem),
+  let αlink := (link_abs final init αbf αaf) in
+  αlink (CL.link_tick final init Cout αlink C (ST mem (L _ _ final af (LINK_pf_af _ _ af))) x v) =
   AL.link_tick (trans_ctx αbf Cout) (trans_ctx αlink C) (Abs.ST abs_mem (AF (αaf af))) x (trans_v αlink v).
 Proof.
-  intros. simpl. rewrite leb_refl. simpl. rewrite leb_refl.
+  intros. simpl. rewrite t_refl. simpl. rewrite t_refl.
   assert (αaf
      (tick
-        (CL.filter_ctx_af final
-           (delete_ctx (fun t t' : CL.link =>
+        (CL.filter_ctx_af final _
+           (delete_ctx (fun t t' : CL.link final init =>
                ALinking.link_eqb (αlink t) (αlink t'))
-               (CL.lift_ctx_bf init Cout) C))
+               (CL.lift_ctx_bf _ init Cout) C))
         (ST
-           (CL.filter_mem_af final
-              (CL.delete_ctx_mem αlink (CL.lift_ctx_bf init Cout) mem)) af) x
-        (CL.filter_v_af final
-           (delete_ctx_v (fun t t' : CL.link =>
+           (CL.filter_mem_af final _
+              (CL.delete_ctx_mem αlink (CL.lift_ctx_bf _ init Cout) mem)) af) x
+        (CL.filter_v_af final _
+           (delete_ctx_v (fun t t' : CL.link final init =>
                ALinking.link_eqb (αlink t) (αlink t'))
-              (CL.lift_ctx_bf init Cout) v))) =
+              (CL.lift_ctx_bf _ init Cout) v))) =
       Abstract.tick
      (AL.filter_ctx_af
         (delete_ctx AL.link_eqb (AL.lift_ctx_bf (trans_ctx αbf Cout))
@@ -290,11 +191,11 @@ Proof.
     split; try reflexivity. apply trans_mem_link; eauto.
     destruct v; simpl in *.
     replace (trans_ctx αaf
-      (CL.filter_ctx_af final
+      (CL.filter_ctx_af final init
         (delete_ctx
-           (fun t t' : CL.link =>
+           (fun t t' : CL.link final init =>
             ALinking.link_eqb (αlink t) (αlink t'))
-           (CL.lift_ctx_bf init Cout) C0))) with
+           (CL.lift_ctx_bf final init Cout) C0))) with
       (AL.filter_ctx_af
       (delete_ctx AL.link_eqb (AL.lift_ctx_bf (trans_ctx αbf Cout))
         (trans_ctx αlink C0))). eauto.
