doc/coq/simple/Linking.v
@@ -1,5 +1,6 @@
 From Simple Require Export Sound.
 Require Export Coq.Logic.FunctionalExtensionality.
+Require Export Coq.Logic.ProofIrrelevance.
 
 Generalizable Variables T BT AT.
 
@@ -21,21 +22,23 @@ Proof.
   eauto. intros. rewrite eqb_eq. eauto.
 Qed.
 
-Inductive link `{Eq BT} `{Eq AT} :=
-  | L (bf : BT) (af : AT)
+Inductive link {BT AT} (final : BT) (init : AT) :=
+  | L bf af 
+      (LINK : (bf <> final -> af = init) /\ 
+              (af <> init -> bf = final))
 .
 
-Definition link_eqb `{EB : Eq BT} `{EA : Eq AT} 
-  (t1 : @link BT EB AT EA) (t2 : @link BT EB AT EA) :=
+Definition link_eqb `{Eq BT} `{Eq AT} (final : BT) (init : AT)
+  (t1 : link final init) (t2 : link final init) :=
   match t1, t2 with
-  | L bf af, L bf' af' =>
+  | L _ _ bf af _, L _ _ bf' af' _ =>
     eqb bf bf' && eqb af af'
   end.
 
-Definition link_leb `{EB : Eq BT} `{@OrderT BT EB} `{EA : Eq AT} `{@OrderT AT EA} 
-  (t1 : @link BT EB AT EA) (t2 : @link BT EB AT EA) :=
+Definition link_leb `{OrderT BT} `{OrderT AT} (final : BT) (init : AT) 
+  (t1 : link final init) (t2 : link final init) :=
   match t1, t2 with
-  | L bf af, L bf' af' =>
+  | L _ _ bf af _, L _ _ bf' af' _ =>
     if leb bf bf' then
       if eqb bf bf' then
         leb af af'
@@ -43,11 +46,8 @@ Definition link_leb `{EB : Eq BT} `{@OrderT BT EB} `{EA : Eq AT} `{@OrderT AT EA
     else false
   end.
 
-Lemma link_leb_refl : 
-  forall 
-    `{EB : Eq BT} `{EA : Eq AT}
-    `{OB : @OrderT BT EB} `{OA : @OrderT AT EA} t,
-  @link_leb BT EB OB AT EA OA t t = true.
+Lemma link_leb_refl `{OrderT BT} `{OrderT AT} (final : BT) (init : AT) : 
+  forall t, link_leb final init t t = true.
 Proof.
   intros. destruct t. simpl. rewrite leb_refl. 
   replace (eqb bf bf) with true.
@@ -55,18 +55,15 @@ Proof.
   symmetry. apply eqb_eq. eauto.
 Qed.
 
-Lemma link_leb_trans :
-  forall 
-    `{EB : Eq BT} `{EA : Eq AT}
-    `{OB : @OrderT BT EB} `{OA : @OrderT AT EA}
-    t t' t''
-    (LE : @link_leb BT EB OB AT EA OA t t' = true)
-    (LE' : @link_leb BT EB OB AT EA OA t' t'' = true),
-  link_leb t t'' = true.
+Lemma link_leb_trans `{OrderT BT} `{OrderT AT} (final : BT) (init : AT) :
+  forall t t' t''
+    (LE : link_leb final init t t' = true)
+    (LE' : link_leb final init t' t'' = true),
+  link_leb final init t t'' = true.
 Proof.
   intros.
-  destruct t as [bf af]; destruct t' as [bf' af'];
-  destruct t'' as [bf'' af'']; simpl in *.
+  destruct t as [bf af ?]; destruct t' as [bf' af' ?];
+  destruct t'' as [bf'' af'' ?]; simpl in *.
   destruct (leb bf bf') eqn:LEbf;
   destruct (leb bf' bf'') eqn:LEbf';
   try (inversion LE; fail);
@@ -91,16 +88,14 @@ Proof.
     apply EQbf. apply leb_sym; eauto.
 Qed.
 
-Lemma link_leb_sym :
-  forall 
-    `{EB : Eq BT} `{EA : Eq AT}
-    `{OB : @OrderT BT EB} `{OA : @OrderT AT EA} t t'
-    (LE : @link_leb BT EB OB AT EA OA t t' = true)
-    (LE' : @link_leb BT EB OB AT EA OA t' t = true),
+Lemma link_leb_sym `{OrderT BT} `{OrderT AT} (final : BT) (init : AT) :
+  forall t t'
+    (LE : link_leb final init t t' = true)
+    (LE' : link_leb final init t' t = true),
   t = t'.
 Proof.
   intros.
-  destruct t as [bf af]; destruct t' as [bf' af'];
+  destruct t as [bf af ?]; destruct t' as [bf' af' ?];
   simpl in *;
   destruct (leb bf bf') eqn:LEbf;
   destruct (leb bf' bf) eqn:LEbf';
@@ -112,19 +107,19 @@ Proof.
   replace (eqb bf bf) with true in *.
   assert (af = af').
   apply leb_sym; eauto. subst; eauto.
+  assert (LINK = LINK0) as RR. apply proof_irrelevance.
+  rewrite RR. eauto.
   symmetry. apply eqb_eq. eauto.
 Qed.
 
-Lemma link_leb_or :
-  forall 
-    `{EB : Eq BT} `{EA : Eq AT}
-    `{OB : @OrderT BT EB} `{OA : @OrderT AT EA} t t',
-  let le1 := @link_leb BT EB OB AT EA OA t t' in
-  let le2 := @link_leb BT EB OB AT EA OA t' t in
+Lemma link_leb_or `{OrderT BT} `{OrderT AT} (final : BT) (init : AT) :
+  forall t t',
+  let le1 := link_leb final init t t' in
+  let le2 := link_leb final init t' t in
   le1 || le2 = true.
 Proof.
   intros.
-  destruct t as [bf af]; destruct t' as [bf' af'].
+  destruct t as [bf af ?]; destruct t' as [bf' af' ?].
   simpl in *.
   destruct (leb bf bf') eqn:LEbf;
   destruct (leb bf' bf) eqn:LEbf';
@@ -146,269 +141,272 @@ Proof.
     inversion contra.
 Qed.
 
-Lemma link_eqb_eq :
-  forall `{EB : Eq BT} `{EA : Eq AT} t t',
-  @link_eqb BT EB AT EA t t' = true <-> t = t'.
+Lemma link_eqb_eq `{Eq BT} `{Eq AT} (final : BT) (init : AT):
+  forall t t', link_eqb final init t t' = true <-> t = t'.
 Proof.
   intros.
-  destruct t as [bf af]; destruct t' as [bf' af'];
+  destruct t as [bf af LINK]; destruct t' as [bf' af' LINK'];
   simpl in *;
   split; intro EQ.
   destruct (eqb bf bf') eqn:EQbf;
   destruct (eqb af af') eqn:EQaf;
   try (inversion EQ; fail).
   rewrite eqb_eq in EQbf.
-  rewrite eqb_eq in EQaf. subst; eauto.
+  rewrite eqb_eq in EQaf. subst.
+  replace LINK with LINK'. eauto. apply proof_irrelevance.
   inversion EQ; subst.
   replace (eqb bf' bf') with true;
   try replace (eqb af' af') with true;
   eauto; symmetry; apply eqb_eq; eauto.
 Qed.
 
-Lemma link_eqb_neq :
-  forall `{EB : Eq BT} `{EA : Eq AT} t t',
-  @link_eqb BT EB AT EA t t' = false <-> t <> t'.
+Lemma link_eqb_neq `{Eq BT} `{Eq AT} (final : BT) (init : AT):
+  forall t t', link_eqb final init t t' = false <-> t <> t'.
 Proof.
   intros.
   split; intro NEQ.
   red. intros EQ.
-  assert (link_eqb t t' = true) as RR. apply link_eqb_eq. eauto.
+  assert (link_eqb final init t t' = true) as RR. apply link_eqb_eq. eauto.
   rewrite RR in NEQ. inversion NEQ.
   refl_bool. intros contra. rewrite link_eqb_eq in contra.
   apply NEQ; eauto.
 Qed.
 
-#[export] Instance LinkEq `{EB : Eq BT} `{EA : Eq AT} :
-  Eq (@link BT EB AT EA) :=
+#[export] Instance LinkEq `{Eq BT} `{Eq AT} (final : BT) (init : AT) :
+  Eq (link final init) :=
 {
-  eqb := link_eqb;
-  eqb_eq := link_eqb_eq;
-  eqb_neq := link_eqb_neq
+  eqb := link_eqb final init;
+  eqb_eq := link_eqb_eq final init;
+  eqb_neq := link_eqb_neq final init
 }.
 
-#[export] Instance LinkOrderT `{EB : Eq BT} `{EA : Eq AT} `{OB : @OrderT BT EB} `{OA : @OrderT AT EA} :
-  @OrderT (@link BT EB AT EA) LinkEq :=
+#[export] Instance LinkOrderT `{OrderT BT} `{OrderT AT} (final : BT) (init : AT) :
+  @OrderT (link final init) (LinkEq final init) :=
   {
-    leb := link_leb;
-    leb_refl := link_leb_refl;
-    leb_trans := link_leb_trans;
-    leb_sym := link_leb_sym;
-    leb_or := link_leb_or
+    leb := link_leb final init;
+    leb_refl := link_leb_refl final init;
+    leb_trans := link_leb_trans final init;
+    leb_sym := link_leb_sym final init;
+    leb_or := link_leb_or final init
   }.
 
 Fixpoint filter_ctx_bf
-  `{OrderT BT} `{EA : Eq AT} (final : BT)
-  (C : @dy_ctx (@link BT _ AT EA)) :=
+  `{OrderT BT} `{EA : Eq AT} (final : BT) (init : AT)
+  (C : @dy_ctx (link final init)) :=
   match C with
   | ([||]) => ([||])
-  | dy_binde x (L bf af) C' =>
-    let filtered := filter_ctx_bf final C' in
-    if leb final bf then filtered else dy_binde x bf filtered
+  | dy_binde x (L _ _ bf af _) C' =>
+    let filtered := filter_ctx_bf final init C' in
+    if eqb final bf then filtered else dy_binde x bf filtered
   | dy_bindm M C' C'' =>
-    dy_bindm M (filter_ctx_bf final C') (filter_ctx_bf final C'')
+    dy_bindm M (filter_ctx_bf final init C') (filter_ctx_bf final init C'')
   end.
 
 Fixpoint filter_ctx_af
-  `{OrderT BT} `{EA : Eq AT} (final : BT)
-  (C : @dy_ctx (@link BT _ AT EA)) :=
+  `{OrderT BT} `{EA : Eq AT} (final : BT) (init : AT)
+  (C : @dy_ctx (link final init)) :=
   match C with
   | ([||]) => ([||])
-  | dy_binde x (L bf af) C' =>
-    let filtered := filter_ctx_af final C' in
-    if leb final bf then dy_binde x af filtered else filtered
+  | dy_binde x (L _ _ bf af _) C' =>
+    let filtered := filter_ctx_af final init C' in
+    if eqb final bf then dy_binde x af filtered else filtered
   | dy_bindm M C' C'' =>
-    dy_bindm M (filter_ctx_af final C') (filter_ctx_af final C'')
+    dy_bindm M (filter_ctx_af final init C') (filter_ctx_af final init C'')
   end.
 
 Definition filter_v_bf 
-  `{OrderT BT} `{EA : Eq AT} (final : BT)
-  (v : @expr_value (@link BT _ AT EA)) :=
+  `{OrderT BT} `{EA : Eq AT} (final : BT) (init : AT)
+  (v : @expr_value (link final init)) :=
   match v with
-  | Closure x e C => Closure x e (filter_ctx_bf final C)
+  | Closure x e C => Closure x e (filter_ctx_bf final init C)
   end.
 
 Definition filter_v_af
-  `{OrderT BT} `{EA : Eq AT} (final : BT)
-  (v : @expr_value (@link BT _ AT EA)) :=
+  `{OrderT BT} `{EA : Eq AT} (final : BT) (init : AT)
+  (v : @expr_value (link final init)) :=
   match v with
-  | Closure x e C => Closure x e (filter_ctx_af final C)
+  | Closure x e C => Closure x e (filter_ctx_af final init C)
   end.
+
+Lemma LINK_pf_bf {BT AT} (final : BT) (init : AT):
+  forall (t : BT),
+    (t <> final -> init = init) /\ (init <> init -> t = final).
+Proof. split; eauto. intros; contradict. Qed.
+
+Lemma LINK_pf_af {BT AT} (final : BT) (init : AT):
+  forall (t : AT),
+    (final <> final -> t = init) /\ (t <> init -> final = final).
+Proof. split; eauto. intros; contradict. Qed.
 
 Definition filter_mem_bf
   `{OrderT BT} `{EA : Eq AT} (final : BT) (init : AT)
-  (mem : (@link BT _ AT EA) -> option (@expr_value (@link BT _ AT EA))) :=
+  (mem : (link final init) -> option (@expr_value (link final init))) :=
   fun t =>
-    match mem (L t init) with
-    | Some v => Some (filter_v_bf final v)
+    match mem (L _ _ t init (LINK_pf_bf final init t)) with
+    | Some v => Some (filter_v_bf final init v)
     | None => None
     end.
 
 Definition filter_mem_af
-  `{OrderT BT} `{EA : Eq AT} (final : BT)
-  (mem : (@link BT _ AT EA) -> option (@expr_value (@link BT _ AT EA))) :=
+  `{OrderT BT} `{EA : Eq AT} (final : BT) (init : AT)
+  (mem : (link final init) -> option (@expr_value (link final init))) :=
   fun t =>
-    match mem (L final t) with
-    | Some v => Some (filter_v_af final v)
+    match mem (L _ _ final t (LINK_pf_af final init t)) with
+    | Some v => Some (filter_v_af final init v)
     | None => None
     end.
 
-Fixpoint lift_ctx_bf `{EB : Eq BT} `{EA : Eq AT} (init : AT) (C : @dy_ctx BT)
-  : @dy_ctx (@link BT EB AT EA) :=
+Fixpoint lift_ctx_bf `{Eq BT} `{Eq AT} (final : BT) (init : AT) (C : @dy_ctx BT)
+  : @dy_ctx (link final init) :=
   match C with
   | ([||]) => ([||])
-  | dy_binde x t C' => dy_binde x (L t init) (lift_ctx_bf init C')
-  | dy_bindm M C' C'' => dy_bindm M (lift_ctx_bf init C') (lift_ctx_bf init C'')
+  | dy_binde x t C' => dy_binde x (L _ _ t init (LINK_pf_bf final init t)) (lift_ctx_bf final init C')
+  | dy_bindm M C' C'' => dy_bindm M (lift_ctx_bf final init C') (lift_ctx_bf final init C'')
   end.
 
-Fixpoint lift_ctx_af `{EB : Eq BT} `{EA : Eq AT} (final : BT) (C : @dy_ctx AT)
-  : @dy_ctx (@link BT EB AT EA) :=
+Fixpoint lift_ctx_af `{Eq BT} `{Eq AT} (final : BT) (init : AT) (C : @dy_ctx AT)
+  : @dy_ctx (link final init) :=
   match C with
   | ([||]) => ([||])
-  | dy_binde x t C' => dy_binde x (L final t) (lift_ctx_af final C')
-  | dy_bindm M C' C'' => dy_bindm M (lift_ctx_af final C') (lift_ctx_af final C'')
+  | dy_binde x t C' => dy_binde x (L _ _ final t (LINK_pf_af final init t)) (lift_ctx_af final init C')
+  | dy_bindm M C' C'' => dy_bindm M (lift_ctx_af final init C') (lift_ctx_af final init C'')
   end.
 
-Definition lift_v_af `{EB : Eq BT} `{EA : Eq AT} (final : BT) (v : @expr_value AT)
-  : @expr_value (@link BT EB AT EA) :=
+Definition lift_v_af `{Eq BT} `{Eq AT} (final : BT) (init : AT) (v : @expr_value AT)
+  : @expr_value (link final init) :=
   match v with
-  | Closure x e C => Closure x e (lift_ctx_af final C)
+  | Closure x e C => Closure x e (lift_ctx_af final init C)
   end.
 
-Definition link_tick `{time BT} `{time AT} `{Eq T}
-  (α : @link BT _ AT _ -> T) (final : BT) (init : AT) (Cout : @dy_ctx BT)
+Definition link_tick `{time BT} `{time AT} (final : BT) (init : AT) (Cout : @dy_ctx BT)
+  `{Eq T} (α : link final init -> T)
   C st x v :=
   match st with
-  | ST mem (L bf af) =>
-    if leb final bf then
-      let Cout := lift_ctx_bf init Cout in
+  | ST mem (L _ _ bf af _) =>
+    if eqb final bf then
+      let Cout := lift_ctx_bf final init Cout in
       let eqb' t t' := eqb (α t) (α t') in
-      L bf
-        (tick (filter_ctx_af final (delete_ctx eqb' Cout C))
-              (ST (filter_mem_af final (delete_ctx_mem α Cout mem)) af)
-              x (filter_v_af final (delete_ctx_v eqb' Cout v)))
+      let af' := 
+        tick (filter_ctx_af final init (delete_ctx eqb' Cout C))
+             (ST (filter_mem_af final init (delete_ctx_mem α Cout mem)) af)
+             x (filter_v_af final init (delete_ctx_v eqb' Cout v)) in
+      L final init final af' (LINK_pf_af final init af')
     else
-      let bf' := tick (filter_ctx_bf final C)
+      let bf' := tick (filter_ctx_bf final init C)
                       (ST (filter_mem_bf final init mem) bf)
-                      x (filter_v_bf final v)
-      in 
-      if leb bf' final then L bf' af else L final af
+                      x (filter_v_bf final init v)
+      in L final init bf' init (LINK_pf_bf final init bf')
   end.
 
-Lemma link_tick_lt `{time BT} `{time AT} `{Eq T} (α : @link BT _ AT _ -> T)
-  (final : BT) (init : AT) (Cout : @dy_ctx BT):
-  forall C mem t x v, t < link_tick α final init Cout C (ST mem t) x v.
+Lemma link_tick_lt `{time BT} `{time AT} (final : BT) (init : AT) (Cout : @dy_ctx BT)
+  `{Eq T} (α : link final init -> T):
+  forall C mem t x v, t < link_tick final init Cout α C (ST mem t) x v.
 Proof.
   destruct t; unfold "<"; simpl.
-  destruct (leb final bf) eqn:LE; simpl;
-  try rewrite leb_refl; try rewrite t_refl; simpl.
-  - intros. split; try apply tick_lt.
+  destruct (eqb final bf) eqn:EQ; simpl;
+  try rewrite eqb_eq in EQ; try rewrite eqb_neq in EQ.
+  - intros. subst. rewrite leb_refl. rewrite t_refl. simpl.
+    split; try apply tick_lt.
   - intros.
     destruct (leb
-      (tick (filter_ctx_bf final C)
+      (tick (filter_ctx_bf final init C)
          (ST (filter_mem_bf final init mem) bf) x 
-         (filter_v_bf final v)) final) eqn:LT; simpl.
+         (filter_v_bf final init v)) final) eqn:LT; simpl.
     + replace (leb bf
-      (tick (filter_ctx_bf final C) (ST (filter_mem_bf final init mem) bf)
-        x (filter_v_bf final v))) with true; try (symmetry; apply tick_lt).
+      (tick (filter_ctx_bf final init C) (ST (filter_mem_bf final init mem) bf)
+        x (filter_v_bf final init v))) with true; try (symmetry; apply tick_lt).
       replace (eqb bf
-      (tick (filter_ctx_bf final C) (ST (filter_mem_bf final init mem) bf)
-        x (filter_v_bf final v))) with false; try (symmetry; apply tick_lt).
+      (tick (filter_ctx_bf final init C) (ST (filter_mem_bf final init mem) bf)
+        x (filter_v_bf final init v))) with false; try (symmetry; apply tick_lt).
       eauto.
-    + assert (eqb bf final = false) as RR.
-      { refl_bool. intros contra. rewrite eqb_eq in contra.
-        subst. rewrite leb_refl in LE. inversion LE. }
-      rewrite RR. split; try reflexivity.
-      assert (leb bf final = true) as RR'.
-      { destruct (leb bf final) eqn:contra; try reflexivity.
-        exfalso.
-        assert (leb final bf || leb bf final = true) as contra'.
-        apply leb_or. rewrite contra in contra'. rewrite LE in contra'. inversion contra'. }
-      rewrite RR'. eauto.
+    + replace (leb bf
+      (tick (filter_ctx_bf final init C) (ST (filter_mem_bf final init mem) bf)
+        x (filter_v_bf final init v))) with true; try (symmetry; apply tick_lt).
+      replace (eqb bf
+      (tick (filter_ctx_bf final init C) (ST (filter_mem_bf final init mem) bf)
+        x (filter_v_bf final init v))) with false; try (symmetry; apply tick_lt).
+      eauto.
 Qed.
 
-#[export] Instance link_time `{time BT} `{time AT} `{Eq T} (α : @link BT _ AT _ -> T) (final : BT) (init : AT) (Cout : @dy_ctx BT) : (@time (@link BT _ AT _) _ _) :=
+#[export] Instance link_time `{time BT} `{time AT} (final : BT) (init : AT) (Cout : @dy_ctx BT) `{Eq T} (α : link final init -> T) : (@time (link final init) _ _) :=
   {
-    tick := link_tick α final init Cout;
-    tick_lt := link_tick_lt α final init Cout
+    tick := link_tick final init Cout α;
+    tick_lt := link_tick_lt final init Cout α
   }.
 
 Definition link_mem `{OrderT BT} `{Eq AT}
   (bmem : BT -> option (@expr_value BT)) (final : BT) (init : AT) (Cout : @dy_ctx BT)
-  (amem : AT -> option (@expr_value AT)) : (@link BT _ AT _) -> option expr_value :=
+  (amem : AT -> option (@expr_value AT)) : (link final init) -> option expr_value :=
   fun t =>
     match t with
-    | L bf af =>
+    | L _ _ bf af _ =>
       if eqb final bf then
-        let Cout := lift_ctx_bf init Cout in
+        let Cout := lift_ctx_bf final init Cout in
         match amem af with
-        | Some (Closure x e C) => Some (Closure x e (Cout<|lift_ctx_af final C|>))
+        | Some (Closure x e C) => Some (Closure x e (Cout<|lift_ctx_af final init C|>))
         | None => None
         end
-      else if leb bf final && eqb af init then
-        match bmem bf with
-        | Some (Closure x e C) => Some (Closure x e (lift_ctx_bf init C))
+      else match bmem bf with
+        | Some (Closure x e C) => Some (Closure x e (lift_ctx_bf final init C))
         | None => None
         end
-      else None
     end.
 
-Lemma filter_lift_eq_af `{time BT} `{time AT} (final : BT):
+Lemma filter_lift_eq_af `{time BT} `{time AT} (final : BT) (init : AT):
   forall (C : @dy_ctx AT),
-    filter_ctx_af final (lift_ctx_af final C) = C.
+    filter_ctx_af final init (lift_ctx_af final init C) = C.
 Proof.
-  induction C; simpl; try rewrite IHC; try rewrite leb_refl; eauto.
+  induction C; simpl; try rewrite IHC; try rewrite t_refl; eauto.
   rewrite IHC2. rewrite IHC1. eauto.
 Qed.
 
 Lemma filter_lift_eq_bf `{time BT} `{time AT} (final : BT) (init : AT) :
   forall (C : @dy_ctx BT) (BOUND : dy_ctx_bound C final),
-    filter_ctx_bf final (lift_ctx_bf init C) = C.
+    filter_ctx_bf final init (lift_ctx_bf final init C) = C.
 Proof.
   induction C; intros; simpl in *;
-  try rewrite IHC; try apply BOUND; 
-  try replace (leb final tx) with false; eauto;
+  try rewrite IHC; try apply BOUND;
+  try replace (eqb final tx) with false; eauto;
   try destruct BOUND as [[LE NEQ] BOUND];
   try (symmetry; refl_bool; intros contra;
-      assert (final = tx); try apply leb_sym; try apply contra; try apply LE;
-      subst; rewrite t_refl in NEQ; inversion NEQ).
+      rewrite eqb_eq in contra; subst; rewrite t_refl in NEQ; inversion NEQ).
   rewrite IHC2; try rewrite IHC1; eauto; apply BOUND.
 Qed.
 
-Lemma filter_delete_eq `{time BT} `{time AT} `{Eq T} (α : @link BT _ AT _ -> T) (final : BT) (init : AT) (Cout : @dy_ctx BT):
+Lemma filter_delete_eq `{time BT} `{time AT} (final : BT) (init : AT) (Cout : @dy_ctx BT) `{Eq T} (α : link final init -> T) :
   forall bmem amem,
-  filter_mem_af final
-    (delete_ctx_mem α (lift_ctx_bf init Cout)
+  filter_mem_af final init
+    (delete_ctx_mem α (lift_ctx_bf final init Cout)
     (link_mem bmem final init Cout amem)) = amem.
 Proof.
   intros. apply functional_extensionality.
   intros. unfold filter_mem_af.
   unfold delete_ctx_mem. simpl. rewrite t_refl.
-  remember (lift_ctx_bf init Cout) as vout eqn:E. clear E.
+  remember (lift_ctx_bf final init Cout) as vout eqn:E. clear E.
   remember (amem x) as o eqn:E. clear E.
   destruct o; eauto. destruct e. simpl.
   rewrite delete_inject_eq. rewrite filter_lift_eq_af. eauto.
   intros. rewrite eqb_eq. eauto.
 Qed.
 
-Lemma link_tick_eq `{time BT} `{time AT} `{Eq T} (α : @link BT _ AT _-> T) (final : BT) (init : AT) (Cout : @dy_ctx BT) :
+Lemma link_tick_eq `{time BT} `{time AT} (final : BT) (init : AT) (Cout : @dy_ctx BT) `{Eq T} (α : link final init -> T) :
   forall bmem C amem t x v,
-    link_tick α final init Cout ((lift_ctx_bf init Cout)<|(lift_ctx_af final C)|>)
-                (ST (link_mem bmem final init Cout amem) (L final t)) x 
-                (inject_ctx_v (lift_ctx_bf init Cout) (lift_v_af final v)) =
-    L final (tick C (ST amem t) x v).
+    link_tick final init Cout α ((lift_ctx_bf final init Cout)<|(lift_ctx_af final init C)|>)
+              (ST (link_mem bmem final init Cout amem) (L final init final t (LINK_pf_af final init t))) x 
+              (inject_ctx_v (lift_ctx_bf final init Cout) (lift_v_af final init v)) =
+    L final init final (tick C (ST amem t) x v) (LINK_pf_af final init (tick C (ST amem t) x v)).
 Proof.
   intros. destruct v. unfold inject_ctx_v. simpl.
   rewrite delete_inject_eq; try (intros; rewrite eqb_eq; eauto).
   rewrite delete_inject_eq; try (intros; rewrite eqb_eq; eauto).
   rewrite filter_delete_eq.
-  rewrite filter_lift_eq_af. rewrite filter_lift_eq_af.
-  rewrite leb_refl.
+  rewrite filter_lift_eq_af. rewrite filter_lift_eq_af. rewrite t_refl.
   reflexivity.
 Qed.
 
-Lemma link_update_m_eq `{time BT} `{time AT} (final : BT) (init : AT) (Cout : @dy_ctx BT):
+Lemma link_update_m_eq `{time BT} `{time AT} (final : BT) (init : AT) (Cout : @dy_ctx BT) :
   forall bmem amem t v (BOUND : time_bound Cout (ST bmem final)),
-  (L final t !-> inject_ctx_v (lift_ctx_bf init Cout) (lift_v_af final v);
+  (L final init final t (LINK_pf_af final init t) !-> inject_ctx_v (lift_ctx_bf final init Cout) (lift_v_af final init v);
     (link_mem bmem final init Cout amem)) =
     link_mem bmem final init Cout (t !-> v; amem).
 Proof.
@@ -423,11 +421,11 @@ Proof.
   rewrite eqb_neq in EQb. contradict.
 Qed.
 
-Lemma lift_addr_x `{time BT} `{time AT} (final : BT) :
+Lemma lift_addr_x `{time BT} `{time AT} (final : BT) (init :AT) :
   forall (C : @dy_ctx AT) x,
-    addr_x (lift_ctx_af final C) x =
+    addr_x (lift_ctx_af final init C) x =
       match addr_x C x with
-      | Some addr => Some (L final addr)
+      | Some addr => Some (L final init final addr (LINK_pf_af final init addr))
       | None => None
       end.
 Proof.
@@ -437,11 +435,11 @@ Proof.
   destruct (addr_x C x0); eauto.
 Qed.
 
-Lemma lift_ctx_M `{time BT} `{time AT} (final : BT) :
+Lemma lift_ctx_M `{time BT} `{time AT} (final : BT) (init : AT) :
   forall (C : @dy_ctx AT) M,
-    ctx_M (lift_ctx_af final C) M =
+    ctx_M (lift_ctx_af final init C) M =
       match ctx_M C M with
-      | Some CM => Some (lift_ctx_af final CM)
+      | Some CM => Some (lift_ctx_af final init CM)
       | None => None
       end.
 Proof.
@@ -451,33 +449,33 @@ Proof.
   destruct (ctx_M C2 M0); eauto.
 Qed.
 
-Lemma lift_plugin_af `{time BT} `{time AT} (final : BT) :
+Lemma lift_plugin_af `{time BT} `{time AT} (final : BT) (init : AT) :
   forall (C C' : @dy_ctx AT),
-    lift_ctx_af final (C[|C'|]) = (lift_ctx_af final C [|lift_ctx_af final C'|]).
+    lift_ctx_af final init (C[|C'|]) = (lift_ctx_af final init C [|lift_ctx_af final init C'|]).
 Proof.
   induction C; simpl; intros; try rewrite IHC; eauto.
   rewrite IHC2. eauto.
 Qed.
 
-Lemma link_eval_eq `{time BT} `{time AT} `{Eq T} (α : @link BT _ AT _ -> T) (final : BT) (init : AT) (Cout : @dy_ctx BT) :
+Lemma link_eval_eq `{time BT} `{time AT} (final : BT) (init : AT) (Cout : @dy_ctx BT) `{Eq T} (α : link final init -> T) :
   forall bmem (BOUND : time_bound Cout (ST bmem final))
          C st e v st'
          (EVAL : @EvalR AT _ _ _ C st e v st'),
-    let inject_C := (lift_ctx_bf init Cout) <|(lift_ctx_af final C)|> in
+    let inject_C := (lift_ctx_bf final init Cout) <|(lift_ctx_af final init C)|> in
     let inject_v :=
       match v with
-      | EVal ev => EVal (inject_ctx_v (lift_ctx_bf init Cout) (lift_v_af final ev))
-      | MVal C_v => MVal ((lift_ctx_bf init Cout)<|(lift_ctx_af final C_v)|>)
+      | EVal ev => EVal (inject_ctx_v (lift_ctx_bf final init Cout) (lift_v_af final init ev))
+      | MVal C_v => MVal ((lift_ctx_bf final init Cout)<|(lift_ctx_af final init C_v)|>)
       end in
     let inject_st :=
       match st with
-      | ST amem t => ST (link_mem bmem final init Cout amem) (L final t)
+      | ST amem t => ST (link_mem bmem final init Cout amem) (L _ _ final t (LINK_pf_af final init t))
       end in
     let inject_st' :=
       match st' with
-      | ST amem' t' => ST (link_mem bmem final init Cout amem') (L final t')
+      | ST amem' t' => ST (link_mem bmem final init Cout amem') (L _ _ final t' (LINK_pf_af final init t'))
       end in
-    @EvalR (@link BT _ AT _) _ _ (link_time α final init Cout)
+    @EvalR (link final init) _ _ (link_time final init Cout α)
       inject_C inject_st e inject_v inject_st'.
 Proof.
   intros. induction EVAL;
@@ -487,55 +485,57 @@ Proof.
   try (destruct inject_st' eqn:INJst'; inversion INJst'; subst); eauto.
   - inversion STATE; subst.
     eapply Eval_var_e; eauto.
-    pose proof (inject_ctx_addr_x x (lift_ctx_bf init Cout) (lift_ctx_af final C)) as RR.
+    pose proof (inject_ctx_addr_x x (lift_ctx_bf final init Cout) (lift_ctx_af final init C)) as RR.
     rewrite lift_addr_x in RR.
     rewrite <- ADDR in RR. symmetry. apply RR.
     unfold link_mem. rewrite t_refl.
     rewrite <- ACCESS. eauto.
   - destruct st_v. destruct arg.
     eapply Eval_app. apply IHEVAL1. apply IHEVAL2.
-    pose proof (link_tick_eq α final init Cout bmem C mem t x (Closure x1 e3 C1)) as RR.
+    pose proof (link_tick_eq final init Cout α bmem C mem t x (Closure x1 e3 C1)) as RR.
     simpl in *. subst inject_C.
     rewrite RR. clear RR.
     pose proof (link_update_m_eq final init Cout bmem mem t (Closure x1 e3 C1) BOUND) as RR. simpl in RR.
     rewrite RR. clear RR.
-    replace (dy_binde x (L final t) ([||])) with (map_inject (lift_ctx_bf init Cout) (dy_binde x (L final t) ([||]))) by reflexivity.
+    replace (dy_binde x (L _ _ final t _) ([||])) with 
+    (map_inject (lift_ctx_bf final init Cout) (dy_binde x (L _ _ final t (LINK_pf_af _ _ t)) ([||]))) by reflexivity.
     rewrite plugin_inject_assoc. rewrite lift_plugin_af in IHEVAL3. eauto.
-  - pose proof (inject_ctx_ctx_M M (lift_ctx_bf init Cout) (lift_ctx_af final C)) as RR.
+  - pose proof (inject_ctx_ctx_M M (lift_ctx_bf final init Cout) (lift_ctx_af final init C)) as RR.
     rewrite lift_ctx_M in RR.
     rewrite <- ACCESS in RR.
     eapply Eval_var_m; eauto.
   - eapply Eval_lete; eauto.
-    pose proof (link_tick_eq α final init Cout bmem C mem t x (Closure x0 e0 C0)) as RR.
+    pose proof (link_tick_eq final init Cout α bmem C mem t x (Closure x0 e0 C0)) as RR.
     simpl in *. subst inject_C.
     rewrite RR. clear RR.
     pose proof (link_update_m_eq final init Cout bmem mem t (Closure x0 e0 C0) BOUND) as RR. simpl in RR.
     rewrite RR. clear RR.
-    replace (dy_binde x (L final t) ([||])) with (map_inject (lift_ctx_bf init Cout) (dy_binde x (L final t) ([||]))) by reflexivity.
+    replace (dy_binde x (L _ _ final t _) ([||])) with 
+    (map_inject (lift_ctx_bf final init Cout) (dy_binde x (L _ _ final t (LINK_pf_af _ _ t)) ([||]))) by reflexivity.
     rewrite plugin_inject_assoc. rewrite lift_plugin_af in IHEVAL2. eauto.
   - eapply Eval_letm; eauto.
-    assert (inject_C [|dy_bindm M (lift_ctx_bf init Cout <| lift_ctx_af final C' |>) ([||])|] =
-            (lift_ctx_bf init Cout <| lift_ctx_af final (C [|dy_bindm M C' ([||])|]) |>)) as RR. 
+    assert (inject_C [|dy_bindm M (lift_ctx_bf final init Cout <| lift_ctx_af final init C' |>) ([||])|] =
+            (lift_ctx_bf final init Cout <| lift_ctx_af final init (C [|dy_bindm M C' ([||])|]) |>)) as RR. 
     { subst inject_C. rewrite lift_plugin_af.
       rewrite <- plugin_inject_assoc. simpl. eauto. } 
     rewrite RR. clear RR. simpl in *. exact IHEVAL2.
 Qed.
 
-Lemma link_reach_eq `{time BT} `{time AT} `{Eq T} (α : @link BT _ AT _ -> T) (final : BT) (init : AT) (Cout : @dy_ctx BT) :
+Lemma link_reach_eq `{time BT} `{time AT} `{Eq T} (final : BT) (init : AT) (Cout : @dy_ctx BT) (α : link final init -> T) :
   forall bmem (BOUND : time_bound Cout (ST bmem final))
          C st e C' st' e'
          (REACH : @one_reach AT _ _ _ C st e C' st' e'),
-    let inject_C := (lift_ctx_bf init Cout) <|(lift_ctx_af final C)|> in
-    let inject_C' := (lift_ctx_bf init Cout) <|(lift_ctx_af final C')|> in
+    let inject_C := (lift_ctx_bf final init Cout) <|(lift_ctx_af final init C)|> in
+    let inject_C' := (lift_ctx_bf final init Cout) <|(lift_ctx_af final init C')|> in
     let inject_st :=
       match st with
-      | ST amem t => ST (link_mem bmem final init Cout amem) (L final t)
+      | ST amem t => ST (link_mem bmem final init Cout amem) (L _ _ final t (LINK_pf_af _ _ t))
       end in
     let inject_st' :=
       match st' with
-      | ST amem' t' => ST (link_mem bmem final init Cout amem') (L final t')
+      | ST amem' t' => ST (link_mem bmem final init Cout amem') (L _ _ final t' (LINK_pf_af _ _ t'))
       end in
-    @one_reach (@link BT _ AT _) _ _ (link_time α final init Cout)
+    @one_reach (link _ _) _ _ (link_time final init Cout α)
       inject_C inject_st e inject_C' inject_st' e'.
 Proof.
   intros. destruct REACH; try destruct st.
@@ -548,17 +548,17 @@ Proof.
     destruct st_lam. subst inject_C inject_st inject_C' inject_st'.
     rewrite <- link_update_m_eq; eauto. rewrite lift_plugin_af. rewrite <- plugin_inject_assoc.
     simpl in *.
-    replace (L final (tick C (ST mem t) x arg)) with 
-      (link_tick α final init Cout (lift_ctx_bf init Cout <| lift_ctx_af final C |>)
-        (ST (link_mem bmem final init Cout mem) (L final t)) x (inject_ctx_v (lift_ctx_bf init Cout) (lift_v_af final arg))).
-    apply (@one_appbody (@link BT _ AT _) _ _ (link_time α final init Cout) 
-                        (lift_ctx_bf init Cout <| lift_ctx_af final C |>)
-                        (ST (link_mem bmem final init Cout mem0) (L final t0))
-                        e1 e2 x e (lift_ctx_bf init Cout <| lift_ctx_af final C_lam |>)
-                        (ST (link_mem bmem final init Cout mem1) (L final t1))
-                        (inject_ctx_v (lift_ctx_bf init Cout) (lift_v_af final arg))
-                        (link_mem bmem final init Cout mem) (L final t)). eauto. eauto.
-    destruct arg. simpl. rewrite leb_refl.
+    replace (L _ _ final (tick C (ST mem t) x arg) _) with 
+      (link_tick final init Cout α (lift_ctx_bf final init Cout <| lift_ctx_af final init C |>)
+        (ST (link_mem bmem final init Cout mem) (L _ _ final t (LINK_pf_af _ _ t))) x (inject_ctx_v (lift_ctx_bf final init Cout) (lift_v_af final init arg))).
+    apply (@one_appbody (link final init) _ _ (link_time final init Cout α) 
+                        (lift_ctx_bf _ init Cout <| lift_ctx_af final _ C |>)
+                        (ST (link_mem bmem final init Cout mem0) (L _ _ final t0 (LINK_pf_af _ _ t0)))
+                        e1 e2 x e (lift_ctx_bf _ init Cout <| lift_ctx_af final _ C_lam |>)
+                        (ST (link_mem bmem final init Cout mem1) (L _ _ final t1 (LINK_pf_af _ _ t1)))
+                        (inject_ctx_v (lift_ctx_bf _ init Cout) (lift_v_af final _ arg))
+                        (link_mem bmem final init Cout mem) (L _ _ final t (LINK_pf_af _ _ t))). eauto. eauto.
+    destruct arg. simpl. rewrite t_refl.
     repeat rewrite delete_inject_eq. repeat rewrite filter_delete_eq. repeat rewrite filter_lift_eq_af. eauto.
     intros; rewrite eqb_eq; eauto. intros; rewrite eqb_eq; eauto.
   - apply one_linkl.
@@ -570,16 +570,16 @@ Proof.
     subst inject_C inject_st inject_C' inject_st'.
     rewrite <- link_update_m_eq; eauto. rewrite lift_plugin_af. rewrite <- plugin_inject_assoc.
     simpl in *.
-    replace (L final (tick C (ST mem t) x v)) with 
-      (link_tick α final init Cout (lift_ctx_bf init Cout <| lift_ctx_af final C |>)
-        (ST (link_mem bmem final init Cout mem) (L final t)) x (inject_ctx_v (lift_ctx_bf init Cout) (lift_v_af final v))).
-    apply (@one_leter (@link BT _ AT _) _ _ (link_time α final init Cout) 
-                      (lift_ctx_bf init Cout <| lift_ctx_af final C |>)
-                      (ST (link_mem bmem final init Cout mem0) (L final t0))
+    replace (L _ _ final (tick C (ST mem t) x v) _) with 
+      (link_tick final init Cout α (lift_ctx_bf _ init Cout <| lift_ctx_af final _ C |>)
+        (ST (link_mem bmem final init Cout mem) (L _ _ final t (LINK_pf_af _ _ t))) x (inject_ctx_v (lift_ctx_bf _ init Cout) (lift_v_af final _ v))).
+    apply (@one_leter (link final init) _ _ (link_time final init Cout α) 
+                      (lift_ctx_bf _ init Cout <| lift_ctx_af final _ C |>)
+                      (ST (link_mem bmem final init Cout mem0) (L _ _ final t0 (LINK_pf_af _ _ t0)))
                       x e m 
-                      (inject_ctx_v (lift_ctx_bf init Cout) (lift_v_af final v))
-                      (link_mem bmem final init Cout mem) (L final t)). eauto.
-    destruct v. simpl. rewrite leb_refl.
+                      (inject_ctx_v (lift_ctx_bf _ init Cout) (lift_v_af final _ v))
+                      (link_mem bmem final init Cout mem) (L _ _ final t (LINK_pf_af _ _ t))). eauto.
+    destruct v. simpl. rewrite t_refl.
     repeat rewrite delete_inject_eq. repeat rewrite filter_delete_eq. repeat rewrite filter_lift_eq_af. eauto.
     intros; rewrite eqb_eq; eauto. intros; rewrite eqb_eq; eauto.
   - apply one_letml.
